

Players A, B, C, and D are playing a dice game in which each player rolls a die until they roll a 5. What is the probability that at least 2 players tie for the most rolls attempted before rolling a 5?

Allow " \rightarrow " to denote a difference in attempted rolls between players. Allow groupings of letters to denote

multiple players tying in attempted rolls (e.g. ABC indicates that it took players A, B, and C the same number of rolls to roll a 5).

Possible Outcomes:

Outcome 1: All players tie (1)

1. ABCD

Outcome 2: 1 succeeds, 3 tie (4)

1. $A \rightarrow BCD$
2. $B \rightarrow ACD$
3. $C \rightarrow ABD$
4. $D \rightarrow ABC$

Outcome 3: 2 tie, then 2 tie (6)

1. $AB \rightarrow CD$
2. $AC \rightarrow BD$
3. $AD \rightarrow BC$
4. $BC \rightarrow AD$
5. $BD \rightarrow AC$
6. $CD \rightarrow AB$

Outcome 4: 3 tie, then 1 succeeds (4)

1. $ABC \rightarrow D$
2. $ABD \rightarrow C$
3. $ACD \rightarrow B$
4. $BCD \rightarrow A$

Outcome 5: 1, then 1, then 2 tie (12)

1. $A \rightarrow B \rightarrow CD$
2. $A \rightarrow C \rightarrow BD$
3. $A \rightarrow D \rightarrow BC$
4. $B \rightarrow A \rightarrow CD$
5. $B \rightarrow C \rightarrow AD$
6. $B \rightarrow D \rightarrow AC$
7. $C \rightarrow A \rightarrow BD$
8. $C \rightarrow B \rightarrow AD$
9. $C \rightarrow D \rightarrow AB$
10. $D \rightarrow A \rightarrow BC$
11. $D \rightarrow B \rightarrow AC$
12. $D \rightarrow C \rightarrow AB$

Outcome 6: 1, then 1, then 1, then 1 (24)

1. $A \rightarrow B \rightarrow C \rightarrow D$
2. $A \rightarrow B \rightarrow D \rightarrow C$
3. $A \rightarrow C \rightarrow B \rightarrow D$
4. $A \rightarrow C \rightarrow D \rightarrow B$
5. $A \rightarrow D \rightarrow B \rightarrow C$
6. $A \rightarrow D \rightarrow C \rightarrow B$
7. $B \rightarrow A \rightarrow C \rightarrow D$

8. $B \rightarrow A \rightarrow D \rightarrow C$
9. $B \rightarrow C \rightarrow A \rightarrow D$
10. $B \rightarrow C \rightarrow D \rightarrow A$
11. $B \rightarrow D \rightarrow A \rightarrow C$
12. $B \rightarrow D \rightarrow C \rightarrow A$
13. $C \rightarrow A \rightarrow B \rightarrow D$
14. $C \rightarrow A \rightarrow D \rightarrow B$
15. $C \rightarrow B \rightarrow A \rightarrow D$
16. $C \rightarrow B \rightarrow D \rightarrow A$
17. $C \rightarrow D \rightarrow A \rightarrow B$
18. $C \rightarrow D \rightarrow B \rightarrow A$
19. $D \rightarrow A \rightarrow B \rightarrow C$
20. $D \rightarrow A \rightarrow C \rightarrow B$
21. $D \rightarrow B \rightarrow A \rightarrow C$
22. $D \rightarrow B \rightarrow C \rightarrow A$
23. $D \rightarrow C \rightarrow A \rightarrow B$
24. $D \rightarrow C \rightarrow B \rightarrow A$

Outcome 7: 1, then 2, then 1 (12)

1. $A \rightarrow BC \rightarrow D$
2. $A \rightarrow BD \rightarrow C$
3. $A \rightarrow CD \rightarrow B$
4. $B \rightarrow AC \rightarrow D$
5. $B \rightarrow AD \rightarrow C$
6. $B \rightarrow CD \rightarrow A$
7. $C \rightarrow AB \rightarrow D$
8. $C \rightarrow AD \rightarrow B$
9. $C \rightarrow BD \rightarrow A$
10. $D \rightarrow AB \rightarrow C$
11. $D \rightarrow AC \rightarrow B$
12. $D \rightarrow BC \rightarrow A$

Outcome 8: 2, then 1, then 1 (12)

1. $AB \rightarrow C \rightarrow D$
2. $AB \rightarrow D \rightarrow C$
3. $AC \rightarrow B \rightarrow D$
4. $AC \rightarrow D \rightarrow B$
5. $AD \rightarrow B \rightarrow C$
6. $AD \rightarrow D \rightarrow B$
7. $BC \rightarrow A \rightarrow D$
8. $BC \rightarrow D \rightarrow A$
9. $BD \rightarrow A \rightarrow C$
10. $BD \rightarrow C \rightarrow A$
11. $CD \rightarrow A \rightarrow B$
12. $CD \rightarrow B \rightarrow A$

As shown, each grouping of scenarios (1, 2-5, 6-11, 12-15, 16-27, 28-51, 52-63, 64-75) represents each of the 8 possible outcomes of the game. There are 78 distinct scenarios within this game. The probabilities of each outcome will be calculated below.

Outcome 1: 1234

$$P = \sum_{n=1}^{\infty} \left[\left(\frac{5}{6} \right)^{n-1} \left(\frac{1}{6} \right) \right]^4$$

Outcome 2: 1 → 234

$$P = 4 * \sum_{n=1}^{\infty} \left[\left(\frac{5}{6} \right)^{n-1} \left(\frac{1}{6} \right) \left[\left(\frac{5}{6} \right)^n \right]^3 * \sum_{m=n+1}^{\infty} \left[\left(\frac{5}{6} \right)^{m-n-1} \left(\frac{1}{6} \right) \right]^3 \right]$$

Outcome 3: 12 → 34

$$P = 6 * \sum_{n=1}^{\infty} \left[\left[\left(\frac{5}{6} \right)^{n-1} \left(\frac{1}{6} \right) \right]^2 \left[\left(\frac{5}{6} \right)^n \right]^2 * \sum_{m=n+1}^{\infty} \left[\left(\frac{5}{6} \right)^{m-n-1} \left(\frac{1}{6} \right) \right]^2 \right]$$

Outcome 4: 123 → 4

$$P = 4 * \sum_{n=1}^{\infty} \left[\left[\left(\frac{5}{6} \right)^{n-1} \left(\frac{1}{6} \right) \right]^3 \left(\frac{5}{6} \right)^n * \sum_{m=n+1}^{\infty} \left[\left(\frac{5}{6} \right)^{m-n-1} \left(\frac{1}{6} \right) \right] \right]$$

Outcome 5: 1 → 2 → 34

$$P = 12 * \sum_{n=1}^{\infty} \left[\left(\frac{5}{6} \right)^{n-1} \left(\frac{1}{6} \right) \left[\left(\frac{5}{6} \right)^n \right]^3 * \sum_{m=n+1}^{\infty} \left[\left(\frac{5}{6} \right)^{m-n-1} \left(\frac{1}{6} \right) \left[\left(\frac{5}{6} \right)^{m-n} \right]^2 * \sum_{p=m+1}^{\infty} \left[\left(\frac{5}{6} \right)^{p-m-1} \left(\frac{1}{6} \right) \right]^2 \right] \right]$$

Outcome 6: 1 → 2 → 3 → 4

$$P = 24 * \sum_{n=1}^{\infty} \left[\left(\frac{5}{6} \right)^{n-1} \left(\frac{1}{6} \right) \left[\left(\frac{5}{6} \right)^n \right]^3 * \sum_{m=n+1}^{\infty} \left[\left(\frac{5}{6} \right)^{m-n-1} \left(\frac{1}{6} \right) \left[\left(\frac{5}{6} \right)^{m-n} \right]^2 * \sum_{p=m+1}^{\infty} \left[\left(\frac{5}{6} \right)^{p-m-1} \left(\frac{1}{6} \right) \left(\frac{5}{6} \right)^{p-m} * \sum_{q=p+1}^{\infty} \left(\frac{5}{6} \right)^{q-p-1} \left(\frac{1}{6} \right) \right] \right] \right]$$

Outcome 7: 1 → 23 → 4

$$P = 12 * \sum_{n=1}^{\infty} \left[\left(\frac{5}{6} \right)^{n-1} \left(\frac{1}{6} \right) \left[\left(\frac{5}{6} \right)^n \right]^3 * \sum_{m=n+1}^{\infty} \left[\left(\left(\frac{5}{6} \right)^{m-n-1} \left(\frac{1}{6} \right) \right)^2 \left(\frac{5}{6} \right)^{m-n} * \sum_{p=m+1}^{\infty} \left(\frac{5}{6} \right)^{p-m-1} \left(\frac{1}{6} \right) \right] \right]$$

Outcome 8: 12 → 3 → 4

$$P = 12 * \sum_{n=1}^{\infty} \left[\left[\left(\frac{5}{6} \right)^{n-1} \left(\frac{1}{6} \right) \right]^2 \left[\left(\frac{5}{6} \right)^n \right]^2 * \sum_{m=n+1}^{\infty} \left[\left(\frac{5}{6} \right)^{m-n-1} \left(\frac{1}{6} \right) \left(\frac{5}{6} \right)^{m-n} * \sum_{p=m+1}^{\infty} \left(\frac{5}{6} \right)^{p-m-1} \left(\frac{1}{6} \right) \right] \right]$$

Thus, the sum of outcomes 1-8 is equal to 1:

$$\begin{aligned}
& \sum_{n=1}^{\infty} \left[\left(\frac{5}{6} \right)^{n-1} \left(\frac{1}{6} \right) \right]^4 \\
& + 4 * \sum_{n=1}^{\infty} \left[\left(\frac{5}{6} \right)^{n-1} \left(\frac{1}{6} \right) \left[\left(\frac{5}{6} \right)^n \right]^3 * \sum_{m=n+1}^{\infty} \left[\left(\frac{5}{6} \right)^{m-n-1} \left(\frac{1}{6} \right) \right]^3 \right] \\
& + 6 * \sum_{n=1}^{\infty} \left[\left[\left(\frac{5}{6} \right)^{n-1} \left(\frac{1}{6} \right) \right]^2 \left[\left(\frac{5}{6} \right)^n \right]^2 * \sum_{m=n+1}^{\infty} \left[\left(\frac{5}{6} \right)^{m-n-1} \left(\frac{1}{6} \right) \right]^2 \right] \\
& + 4 * \sum_{n=1}^{\infty} \left[\left[\left(\frac{5}{6} \right)^{n-1} \left(\frac{1}{6} \right) \right]^3 \left(\frac{5}{6} \right)^n * \sum_{m=n+1}^{\infty} \left[\left(\frac{5}{6} \right)^{m-n-1} \left(\frac{1}{6} \right) \right] \right] \\
& + 12 * \sum_{n=1}^{\infty} \left[\left(\frac{5}{6} \right)^{n-1} \left(\frac{1}{6} \right) \left[\left(\frac{5}{6} \right)^n \right]^3 * \sum_{m=n+1}^{\infty} \left[\left(\frac{5}{6} \right)^{m-n-1} \left(\frac{1}{6} \right) \left[\left(\frac{5}{6} \right)^{m-n} \right]^2 \right. \right. \\
& \quad \left. \left. * \sum_{p=m+1}^{\infty} \left[\left(\frac{5}{6} \right)^{p-m-1} \left(\frac{1}{6} \right) \right]^2 \right] \right] \\
& + 24 * \sum_{n=1}^{\infty} \left[\left(\frac{5}{6} \right)^{n-1} \left(\frac{1}{6} \right) \left[\left(\frac{5}{6} \right)^n \right]^3 * \sum_{m=n+1}^{\infty} \left[\left(\frac{5}{6} \right)^{m-n-1} \left(\frac{1}{6} \right) \left[\left(\frac{5}{6} \right)^{m-n} \right]^2 \right. \right. \\
& \quad \left. \left. * \sum_{p=m+1}^{\infty} \left[\left(\frac{5}{6} \right)^{p-m-1} \left(\frac{1}{6} \right) \left(\frac{5}{6} \right)^{p-m} * \sum_{q=p+1}^{\infty} \left(\frac{5}{6} \right)^{q-p-1} \left(\frac{1}{6} \right) \right] \right] \right] \\
& + 12 * \sum_{n=1}^{\infty} \left[\left(\frac{5}{6} \right)^{n-1} \left(\frac{1}{6} \right) \left[\left(\frac{5}{6} \right)^n \right]^3 * \sum_{m=n+1}^{\infty} \left[\left(\left(\frac{5}{6} \right)^{m-n-1} \left(\frac{1}{6} \right) \right)^2 \left(\frac{5}{6} \right)^{m-n} \right. \right. \\
& \quad \left. \left. * \sum_{p=m+1}^{\infty} \left(\frac{5}{6} \right)^{p-m-1} \left(\frac{1}{6} \right) \right] \right] \\
& + 12 * \sum_{n=1}^{\infty} \left[\left[\left(\frac{5}{6} \right)^{n-1} \left(\frac{1}{6} \right) \right]^2 \left[\left(\frac{5}{6} \right)^n \right]^2 * \sum_{m=n+1}^{\infty} \left[\left(\frac{5}{6} \right)^{m-n-1} \left(\frac{1}{6} \right) \left(\frac{5}{6} \right)^{m-n} \right. \right. \\
& \quad \left. \left. * \sum_{p=m+1}^{\infty} \left(\frac{5}{6} \right)^{p-m-1} \left(\frac{1}{6} \right) \right] \right] = 1
\end{aligned}$$

Therefore, the methods are proved and the probability of a tie can be calculated by summing the probabilities

of the scenarios that end in more than one player (scenarios 1, 2, 3, and 5):

$$\begin{aligned}
P = & \sum_{n=1}^{\infty} \left[\left(\frac{5}{6} \right)^{n-1} \left(\frac{1}{6} \right) \right]^4 \\
& + 4 * \sum_{n=1}^{\infty} \left[\left(\frac{5}{6} \right)^{n-1} \left(\frac{1}{6} \right) \left[\left(\frac{5}{6} \right)^n \right]^3 * \sum_{m=n+1}^{\infty} \left[\left(\frac{5}{6} \right)^{m-n-1} \left(\frac{1}{6} \right) \right]^3 \right] \\
& + 6 * \sum_{n=1}^{\infty} \left[\left[\left(\frac{5}{6} \right)^{n-1} \left(\frac{1}{6} \right) \right]^2 \left[\left(\frac{5}{6} \right)^n \right]^2 * \sum_{m=n+1}^{\infty} \left[\left(\frac{5}{6} \right)^{m-n-1} \left(\frac{1}{6} \right) \right]^2 \right] \\
& + 12 * \sum_{n=1}^{\infty} \left[\left(\frac{5}{6} \right)^{n-1} \left(\frac{1}{6} \right) \left[\left(\frac{5}{6} \right)^n \right]^3 * \sum_{m=n+1}^{\infty} \left[\left(\frac{5}{6} \right)^{m-n-1} \left(\frac{1}{6} \right) \left[\left(\frac{5}{6} \right)^{m-n} \right]^2 \right. \right. \\
& \quad \left. \left. * \sum_{p=m+1}^{\infty} \left[\left(\frac{5}{6} \right)^{p-m-1} \left(\frac{1}{6} \right) \right]^2 \right] \right] = \frac{114033471}{1894783891} \approx 6.0183\%
\end{aligned}$$